nola/iris/wp.v
@@ -5,42 +5,287 @@ From iris.bi Require Import fixpoint.
 From iris.proofmode Require Import tactics.
 From nola Require Import fupd.
 
+(** ** What becomes [irisGS_gen] combined with an extra world satisfaction *)
+Class irisGS'_gen (hlc : has_lc) (Λ : language) (Σ : gFunctors) := IrisG' {
+  iris'_invGS :: invGS_gen hlc Σ;
+  state_interp' : state Λ → nat → list (observation Λ) → nat → iProp Σ;
+  fork_post' : val Λ → iProp Σ;
+  num_laters_per_step' : nat → nat;
+  state_interp'_mono σ ns κs nt:
+    state_interp' σ ns κs nt ⊢ |={∅}=> state_interp' σ (S ns) κs nt
+}.
+
+(** [irisGS_gen] made from [irisGS'_gen] and an extra world satisfaction *)
+Program Definition iris_wsat `{!irisGS'_gen hlc Λ Σ}
+  (W : iProp Σ) : irisGS_gen hlc Λ Σ := {|
+  iris_invGS := iris'_invGS;
+  state_interp σ ns ks nt := (W ∗ state_interp' σ ns ks nt)%I;
+  fork_post := fork_post';
+  num_laters_per_step := num_laters_per_step';
+|}.
+Next Obligation. iIntros "* [$ ?]". by iApply state_interp'_mono. Qed.
+
 Local Transparent iris_invGS.
 Local Notation wp_unseal := iris.program_logic.weakestpre.wp_aux.(seal_eq).
 Local Notation twp_unseal :=
   iris.program_logic.total_weakestpre.twp_aux.(seal_eq).
 Local Notation twp_pre' := iris.program_logic.total_weakestpre.twp_pre'.
 
-Section wp.
-  Context `{!invGS_gen hlc Σ} {Λ : language}
-    {fp : val Λ → iProp Σ} {nl : nat → nat}.
+(** ** [wpw]/[twpw]: [wp]/[twp] for [iris_wsat] *)
+Notation wpw W := (@wp _ _ _ _ (@wp' _ _ _ (iris_wsat W))).
+Notation twpw W := (@twp _ _ _ _ (@twp' _ _ _ (iris_wsat W))).
 
-  (** Make the state interpretation explicit in [wp]/[twp] *)
-  Local Notation IrG Φ monoΦ := (IrisG _ Φ fp nl monoΦ).
-  Local Notation wpx Φ monoΦ := (@wp' _ _ _ (IrG Φ monoΦ)).
-  Local Notation twpx Φ monoΦ := (@twp' _ _ _ (IrG Φ monoΦ)).
+Section wpw.
+  Context `{!irisGS'_gen hlc Λ Σ}.
 
-  (** [wp] is non-expansive over the state interpretation *)
-  Lemma wp_ne_interp {Φ Ψ : _ -d> _ -d> _ -d> _ -d> _} {n monoΦ monoΨ} :
-    Φ ≡{n}≡ Ψ → (wpx Φ monoΦ : _ -d> _ -d> _ -d> _ -d> _) ≡{n}≡ wpx Ψ monoΨ.
+  (** [wpw] is non-expansive over the world satisfaction *)
+  Lemma wpw_ne {W W' n s E e Φ Ψ} :
+    W ≡{n}≡ W' → (Φ : _ -d> _) ≡{n}≡ Ψ → wpw W s E e Φ ≡{n}≡ wpw W' s E e Ψ.
   Proof.
-    move=> ΦΨ. rewrite /wp' wp_unseal=> ?. apply fixpoint_ne=> ????.
-    unfold wp_pre=>/=. do 12 f_equiv; [by apply ΦΨ|]. do 13 f_equiv.
-    apply step_fupdN_ne. do 2 f_equiv. apply ΦΨ.
+    move=> ? ΦΨ.
+    enough (go : (wpw W : _ -d> _ -d> _ -d> _ -d> _) ≡{n}≡ wpw W').
+    { etrans; [apply go|]. by f_equiv. }
+    rewrite /wp' wp_unseal=> ?. apply fixpoint_ne=> ????.
+    rewrite /wp_pre /=. do 13 f_equiv; [done|]. do 12 f_equiv.
+    apply step_fupdN_ne. by do 3 f_equiv.
   Qed.
-  Lemma wp_proper_interp {Φ Ψ : _ -d> _ -d> _ -d> _ -d> _} {monoΦ monoΨ} :
-    Φ ≡ Ψ → (wpx Φ monoΦ : _ -d> _ -d> _ -d> _ -d> _) ≡ wpx Ψ monoΨ.
-  Proof. rewrite !equiv_dist=> ??. by apply wp_ne_interp. Qed.
+  Lemma wpw_proper {W W' s E e Φ Ψ} :
+    W ⊣⊢ W' → (Φ : _ -d> _) ≡ Ψ → wpw W s E e Φ ⊣⊢ wpw W' s E e Ψ.
+  Proof. rewrite !equiv_dist=> ???. by apply wpw_ne. Qed.
 
-  (** [twp] is non-expansive over the state interpretation *)
-  Lemma twp_ne_interp {Φ Ψ : _ -d> _ -d> _ -d> _ -d> _} {n monoΦ monoΨ} :
-    Φ ≡{n}≡ Ψ → (twpx Φ monoΦ : _ -d> _ -d> _ -d> _ -d> _) ≡{n}≡ twpx Ψ monoΨ.
+  (** [twpw] is non-expansive over the world satisfaction *)
+  Lemma twpw_ne {W W' n s E e Φ Ψ} :
+    W ≡{n}≡ W' → (Φ : _ -d> _) ≡{n}≡ Ψ → twpw W s E e Φ ≡{n}≡ twpw W' s E e Ψ.
   Proof.
-    move=> ΦΨ. rewrite /twp' twp_unseal=> ????.
+    move=> ? ΦΨ.
+    enough (go : (twpw W : _ -d> _ -d> _ -d> _ -d> _) ≡{n}≡ twpw W').
+    { etrans; [apply go|]. by f_equiv. }
+    rewrite /twp' twp_unseal=> ????.
     apply least_fixpoint_ne; [|done]=> ?[[??]?]. rewrite /twp_pre'/twp_pre/=.
-    do 10 f_equiv; [by apply ΦΨ|]. do 14 f_equiv. apply ΦΨ.
+    do 11 f_equiv; [done|]. by do 14 f_equiv.
   Qed.
-  Lemma twp_proper_interp {Φ Ψ : _ -d> _ -d> _ -d> _ -d> _} {monoΦ monoΨ} :
-    Φ ≡ Ψ → (twpx Φ monoΦ : _ -d> _ -d> _ -d> _ -d> _) ≡ twpx Ψ monoΨ.
-  Proof. rewrite !equiv_dist=> ??. by apply twp_ne_interp. Qed.
-End wp.
+  Lemma twp_proper {W W' s E e Φ Ψ} :
+    W ⊣⊢ W' → (Φ : _ -d> _) ≡ Ψ → twpw W s E e Φ ⊣⊢ twpw W' s E e Ψ.
+  Proof. rewrite !equiv_dist=> ???. by apply twpw_ne. Qed.
+End wpw.
+
+(** Notation for [wpw]/[twpw] *)
+
+Notation "WP[ W ] e @ s ; E {{ Φ } }" := (wpw W s E e%E Φ)
+  (at level 20, e, Φ at level 200, only parsing) : bi_scope.
+Notation "WP[ W ] e @ E {{ Φ } }" := (wpw W NotStuck E e%E Φ)
+  (at level 20, e, Φ at level 200, only parsing) : bi_scope.
+Notation "WP[ W ] e @ E ? {{ Φ } }" := (wpw W MaybeStuck E e%E Φ)
+  (at level 20, e, Φ at level 200, only parsing) : bi_scope.
+Notation "WP[ W ] e {{ Φ } }" := (wpw W NotStuck ⊤ e%E Φ)
+  (at level 20, e, Φ at level 200, only parsing) : bi_scope.
+Notation "WP[ W ] e ? {{ Φ } }" := (wpw W MaybeStuck ⊤ e%E Φ)
+  (at level 20, e, Φ at level 200, only parsing) : bi_scope.
+
+Notation "WP[ W ] e @ s ; E {{ v , Q } }" := (wpw W s E e%E (λ v, Q))
+  (at level 20, e, Q at level 200,
+   format "'[hv' WP[ W ]  e  '/' @  '[' s ;  '/' E  ']' '/' {{  '[' v ,  '/' Q  ']' } } ']'")
+  : bi_scope.
+Notation "WP[ W ] e @ E {{ v , Q } }" := (wpw W NotStuck E e%E (λ v, Q))
+  (at level 20, e, Q at level 200,
+   format "'[hv' WP[ W ]  e  '/' @  E  '/' {{  '[' v ,  '/' Q  ']' } } ']'")
+  : bi_scope.
+Notation "WP[ W ] e @ E ? {{ v , Q } }" := (wpw W MaybeStuck E e%E (λ v, Q))
+  (at level 20, e, Q at level 200,
+   format "'[hv' WP[ W ]  e  '/' @  E  '/' ? {{  '[' v ,  '/' Q  ']' } } ']'")
+  : bi_scope.
+Notation "WP[ W ] e {{ v , Q } }" := (wpw W NotStuck ⊤ e%E (λ v, Q))
+  (at level 20, e, Q at level 200,
+   format "'[hv' WP[ W ]  e  '/' {{  '[' v ,  '/' Q  ']' } } ']'") : bi_scope.
+Notation "WP[ W ] e ? {{ v , Q } }" := (wpw W MaybeStuck ⊤ e%E (λ v, Q))
+  (at level 20, e, Q at level 200,
+   format "'[hv' WP[ W ]  e  '/' ? {{  '[' v ,  '/' Q  ']' } } ']'") : bi_scope.
+
+Notation "{{{ P } } } [ W ] e @ s ; E {{{ x .. y , 'RET' pat ; Q } } }" :=
+  (□ ∀ Φ, P -∗ ▷ (∀ x, .. (∀ y, Q -∗ Φ pat%V) .. ) -∗ WP[W] e @ s; E {{ Φ }})%I
+  (at level 20, x closed binder, y closed binder,
+   format "'[hv' {{{  '[' P  ']' } } } [ W ]  '/  ' e  '/' @  '[' s ;  '/' E  ']' '/' {{{  '[' x  ..  y ,  RET  pat ;  '/' Q  ']' } } } ']'")
+  : bi_scope.
+Notation "{{{ P } } } [ W ] e @ E {{{ x .. y , 'RET' pat ; Q } } }" :=
+  (□ ∀ Φ, P -∗ ▷ (∀ x, .. (∀ y, Q -∗ Φ pat%V) .. ) -∗ WP[W] e @ E {{ Φ }})%I
+  (at level 20, x closed binder, y closed binder,
+   format "'[hv' {{{  '[' P  ']' } } } [ W ]  '/  ' e  '/' @  E  '/' {{{  '[' x  ..  y ,  RET  pat ;  '/' Q  ']' } } } ']'")
+  : bi_scope.
+Notation "{{{ P } } } [ W ] e @ E ? {{{ x .. y , 'RET' pat ; Q } } }" :=
+  (□ ∀ Φ, P -∗ ▷ (∀ x, .. (∀ y, Q -∗ Φ pat%V) .. ) -∗ WP[W] e @ E ?{{ Φ }})%I
+  (at level 20, x closed binder, y closed binder,
+   format "'[hv' {{{  '[' P  ']' } } } [ W ]  '/  ' e  '/' @  E  '/' ? {{{  '[' x  ..  y ,  RET  pat ;  '/' Q  ']' } } } ']'")
+  : bi_scope.
+Notation "{{{ P } } } [ W ] e {{{ x .. y , 'RET' pat ; Q } } }" :=
+  (□ ∀ Φ, P -∗ ▷ (∀ x, .. (∀ y, Q -∗ Φ pat%V) .. ) -∗ WP[W] e {{ Φ }})%I
+  (at level 20, x closed binder, y closed binder,
+   format "'[hv' {{{  '[' P  ']' } } } [ W ]  '/  ' e  '/' {{{  '[' x  ..  y ,  RET  pat ;  '/' Q  ']' } } } ']'")
+  : bi_scope.
+Notation "{{{ P } } } [ W ] e ? {{{ x .. y , 'RET' pat ; Q } } }" :=
+  (□ ∀ Φ, P -∗ ▷ (∀ x, .. (∀ y, Q -∗ Φ pat%V) .. ) -∗ WP[W] e ?{{ Φ }})%I
+  (at level 20, x closed binder, y closed binder,
+   format "'[hv' {{{  '[' P  ']' } } } [ W ]  '/  ' e  '/' ? {{{  '[' x  ..  y ,   RET  pat ;  '/' Q  ']' } } } ']'")
+  : bi_scope.
+
+Notation "{{{ P } } } [ W ] e @ s ; E {{{ 'RET' pat ; Q } } }" :=
+  (□ ∀ Φ, P -∗ ▷ (Q -∗ Φ pat%V) -∗ WP[W] e @ s; E {{ Φ }})%I
+  (at level 20,
+   format "'[hv' {{{  '[' P  ']' } } } [ W ]  '/  ' e  '/' @  '[' s ;  '/' E  ']' '/' {{{  '[' RET  pat ;  '/' Q  ']' } } } ']'")
+  : bi_scope.
+Notation "{{{ P } } } [ W ] e @ E {{{ 'RET' pat ; Q } } }" :=
+  (□ ∀ Φ, P -∗ ▷ (Q -∗ Φ pat%V) -∗ WP[W] e @ E {{ Φ }})%I
+  (at level 20,
+   format "'[hv' {{{  '[' P  ']' } } } [ W ]  '/  ' e  '/' @  E  '/' {{{  '[' RET  pat ;  '/' Q  ']' } } } ']'")
+  : bi_scope.
+Notation "{{{ P } } } [ W ] e @ E ? {{{ 'RET' pat ; Q } } }" :=
+  (□ ∀ Φ, P -∗ ▷ (Q -∗ Φ pat%V) -∗ WP[W] e @ E ?{{ Φ }})%I
+  (at level 20,
+   format "'[hv' {{{  '[' P  ']' } } } [ W ]  '/  ' e  '/' @  E  '/' ? {{{  '[' RET  pat ;  '/' Q  ']' } } } ']'")
+  : bi_scope.
+Notation "{{{ P } } } [ W ] e {{{ 'RET' pat ; Q } } }" :=
+  (□ ∀ Φ, P -∗ ▷ (Q -∗ Φ pat%V) -∗ WP[W] e {{ Φ }})%I
+  (at level 20,
+   format "'[hv' {{{  '[' P  ']' } } } [ W ]  '/  ' e  '/' {{{  '[' RET  pat ;  '/' Q  ']' } } } ']'")
+  : bi_scope.
+Notation "{{{ P } } } [ W ] e ? {{{ 'RET' pat ; Q } } }" :=
+  (□ ∀ Φ, P -∗ ▷ (Q -∗ Φ pat%V) -∗ WP[W] e ?{{ Φ }})%I
+  (at level 20,
+   format "'[hv' {{{  '[' P  ']' } } } [ W ]  '/  ' e  '/' ? {{{  '[' RET  pat ;  '/' Q  ']' } } } ']'")
+  : bi_scope.
+
+Notation "{{{ P } } } [ W ] e @ s ; E {{{ x .. y , 'RET' pat ; Q } } }" :=
+  (∀ Φ, P -∗ ▷ (∀ x, .. (∀ y, Q -∗ Φ pat%V) .. ) -∗ WP[W] e @ s; E {{ Φ }})
+  : stdpp_scope.
+Notation "{{{ P } } } [ W ] e @ E {{{ x .. y , 'RET' pat ; Q } } }" :=
+  (∀ Φ, P -∗ ▷ (∀ x, .. (∀ y, Q -∗ Φ pat%V) .. ) -∗ WP[W] e @ E {{ Φ }})
+  : stdpp_scope.
+Notation "{{{ P } } } [ W ] e @ E ? {{{ x .. y , 'RET' pat ; Q } } }" :=
+  (∀ Φ, P -∗ ▷ (∀ x, .. (∀ y, Q -∗ Φ pat%V) .. ) -∗ WP[W] e @ E ?{{ Φ }})
+  : stdpp_scope.
+Notation "{{{ P } } } [ W ] e {{{ x .. y , 'RET' pat ; Q } } }" :=
+  (∀ Φ, P -∗ ▷ (∀ x, .. (∀ y, Q -∗ Φ pat%V) .. ) -∗ WP[W] e {{ Φ }})
+  : stdpp_scope.
+Notation "{{{ P } } } [ W ] e ? {{{ x .. y , 'RET' pat ; Q } } }" :=
+  (∀ Φ, P -∗ ▷ (∀ x, .. (∀ y, Q -∗ Φ pat%V) .. ) -∗ WP[W] e ?{{ Φ }})
+  : stdpp_scope.
+Notation "{{{ P } } } [ W ] e @ s ; E {{{ 'RET' pat ; Q } } }" :=
+  (∀ Φ, P -∗ ▷ (Q -∗ Φ pat%V) -∗ WP[W] e @ s; E {{ Φ }}) : stdpp_scope.
+Notation "{{{ P } } } [ W ] e @ E {{{ 'RET' pat ; Q } } }" :=
+  (∀ Φ, P -∗ ▷ (Q -∗ Φ pat%V) -∗ WP[W] e @ E {{ Φ }}) : stdpp_scope.
+Notation "{{{ P } } } [ W ] e @ E ? {{{ 'RET' pat ; Q } } }" :=
+  (∀ Φ, P -∗ ▷ (Q -∗ Φ pat%V) -∗ WP[W] e @ E ?{{ Φ }}) : stdpp_scope.
+Notation "{{{ P } } } [ W ] e {{{ 'RET' pat ; Q } } }" :=
+  (∀ Φ, P -∗ ▷ (Q -∗ Φ pat%V) -∗ WP[W] e {{ Φ }}) : stdpp_scope.
+Notation "{{{ P } } } [ W ] e ? {{{ 'RET' pat ; Q } } }" :=
+  (∀ Φ, P -∗ ▷ (Q -∗ Φ pat%V) -∗ WP[W] e ?{{ Φ }}) : stdpp_scope.
+
+Notation "WP[ W ] e @ s ; E [{ Φ } ]" := (twpw W s E e%E Φ)
+  (at level 20, e, Φ at level 200, only parsing) : bi_scope.
+Notation "WP[ W ] e @ E [{ Φ } ]" := (twpw W NotStuck E e%E Φ)
+  (at level 20, e, Φ at level 200, only parsing) : bi_scope.
+Notation "WP[ W ] e @ E ? [{ Φ } ]" := (twpw W MaybeStuck E e%E Φ)
+  (at level 20, e, Φ at level 200, only parsing) : bi_scope.
+Notation "WP[ W ] e [{ Φ } ]" := (twpw W NotStuck ⊤ e%E Φ)
+  (at level 20, e, Φ at level 200, only parsing) : bi_scope.
+Notation "WP[ W ] e ? [{ Φ } ]" := (twpw W MaybeStuck ⊤ e%E Φ)
+  (at level 20, e, Φ at level 200, only parsing) : bi_scope.
+
+(** Notations with binder. *)
+Notation "WP[ W ] e @ s ; E [{ v , Q } ]" := (twpw W s E e%E (λ v, Q))
+  (at level 20, e, Q at level 200,
+   format "'[hv' WP[ W ]  e  '/' @  '[' s ;  '/' E  ']' '/' [{  '[' v ,  '/' Q  ']' } ] ']'")
+  : bi_scope.
+Notation "WP[ W ] e @ E [{ v , Q } ]" := (twpw W NotStuck E e%E (λ v, Q))
+  (at level 20, e, Q at level 200,
+   format "'[hv' WP[ W ]  e  '/' @  E  '/' [{  '[' v ,  '/' Q  ']' } ] ']'")
+  : bi_scope.
+Notation "WP[ W ] e @ E ? [{ v , Q } ]" := (twpw W MaybeStuck E e%E (λ v, Q))
+  (at level 20, e, Q at level 200,
+   format "'[hv' WP[ W ]  e  '/' @  E  '/' ? [{  '[' v ,  '/' Q  ']' } ] ']'")
+  : bi_scope.
+Notation "WP[ W ] e [{ v , Q } ]" := (twpw W NotStuck ⊤ e%E (λ v, Q))
+  (at level 20, e, Q at level 200,
+   format "'[hv' WP[ W ]  e  '/' [{  '[' v ,  '/' Q  ']' } ] ']'") : bi_scope.
+Notation "WP[ W ] e ? [{ v , Q } ]" := (twpw W MaybeStuck ⊤ e%E (λ v, Q))
+  (at level 20, e, Q at level 200,
+   format "'[hv' WP[ W ]  e  '/' ? [{  '[' v ,  '/' Q  ']' } ] ']'") : bi_scope.
+
+(* Texan triples *)
+Notation "[[{ P } ] ] [ W ] e @ s ; E [[{ x .. y , 'RET' pat ; Q } ] ]" :=
+  (□ ∀ Φ, P -∗ (∀ x, .. (∀ y, Q -∗ Φ pat%V) .. ) -∗ WP[W] e @ s; E [{ Φ }])%I
+  (at level 20, x closed binder, y closed binder,
+   format "'[hv' [[{  '[' P  ']' } ] ] [ W ]  '/  ' e  '/' @  '[' s ;  '/' E  ']' '/' [[{  '[hv' x  ..  y ,  RET  pat ;  '/' Q  ']' } ] ] ']'")
+  : bi_scope.
+Notation "[[{ P } ] ] [ W ] e @ E [[{ x .. y , 'RET' pat ; Q } ] ]" :=
+  (□ ∀ Φ, P -∗ (∀ x, .. (∀ y, Q -∗ Φ pat%V) .. ) -∗ WP[W] e @ E [{ Φ }])%I
+  (at level 20, x closed binder, y closed binder,
+   format "'[hv' [[{  '[' P  ']' } ] ] [ W ]  '/  ' e  '/' @  E  '/' [[{  '[hv' x  ..  y ,  RET  pat ;  '/' Q  ']' } ] ] ']'")
+  : bi_scope.
+Notation "[[{ P } ] ] [ W ] e @ E ? [[{ x .. y , 'RET' pat ; Q } ] ]" :=
+  (□ ∀ Φ, P -∗ (∀ x, .. (∀ y, Q -∗ Φ pat%V) .. ) -∗ WP[W] e @ E ?[{ Φ }])%I
+  (at level 20, x closed binder, y closed binder,
+   format "'[hv' [[{  '[' P  ']' } ] ] [ W ]  '/  ' e  '/' @  E  '/' ? [[{  '[hv' x  ..  y ,  RET  pat ;  '/' Q  ']' } ] ] ']'")
+  : bi_scope.
+Notation "[[{ P } ] ] [ W ] e [[{ x .. y , 'RET' pat ; Q } ] ]" :=
+  (□ ∀ Φ, P -∗ (∀ x, .. (∀ y, Q -∗ Φ pat%V) .. ) -∗ WP[W] e [{ Φ }])%I
+  (at level 20, x closed binder, y closed binder,
+   format "'[hv' [[{  '[' P  ']' } ] ] [ W ]  '/  ' e  '/' [[{  '[hv' x  ..  y ,  RET  pat ;  '/' Q  ']' } ] ] ']'")
+  : bi_scope.
+Notation "[[{ P } ] ] [ W ] e ? [[{ x .. y , 'RET' pat ; Q } ] ]" :=
+  (□ ∀ Φ, P -∗ (∀ x, .. (∀ y, Q -∗ Φ pat%V) .. ) -∗ WP[W] e ?[{ Φ }])%I
+  (at level 20, x closed binder, y closed binder,
+   format "'[hv' [[{  '[' P  ']' } ] ] [ W ]  '/  ' e  '/' ? [[{  '[hv' x  ..  y ,   RET  pat ;  '/' Q  ']' } ] ] ']'")
+  : bi_scope.
+
+Notation "[[{ P } ] ] [ W ] e @ s ; E [[{ 'RET' pat ; Q } ] ]" :=
+  (□ ∀ Φ, P -∗ (Q -∗ Φ pat%V) -∗ WP[W] e @ s; E [{ Φ }])%I
+  (at level 20,
+   format "'[hv' [[{  '[' P  ']' } ] ] [ W ]  '/  ' e  '/' @  '[' s ;  '/' E  ']' '/' [[{  '[hv' RET  pat ;  '/' Q  ']' } ] ] ']'")
+  : bi_scope.
+Notation "[[{ P } ] ] [ W ] e @ E [[{ 'RET' pat ; Q } ] ]" :=
+  (□ ∀ Φ, P -∗ (Q -∗ Φ pat%V) -∗ WP[W] e @ E [{ Φ }])%I
+  (at level 20,
+   format "'[hv' [[{  '[' P  ']' } ] ] [ W ]  '/  ' e  '/' @  E  '/' [[{  '[hv' RET  pat ;  '/' Q  ']' } ] ] ']'")
+  : bi_scope.
+Notation "[[{ P } ] ] [ W ] e @ E ? [[{ 'RET' pat ; Q } ] ]" :=
+  (□ ∀ Φ, P -∗ (Q -∗ Φ pat%V) -∗ WP[W] e @ E ?[{ Φ }])%I
+  (at level 20,
+   format "'[hv' [[{  '[' P  ']' } ] ] [ W ]  '/  ' e  '/' @  E  '/' ? [[{  '[hv' RET  pat ;  '/' Q  ']' } ] ] ']'")
+  : bi_scope.
+Notation "[[{ P } ] ] [ W ] e [[{ 'RET' pat ; Q } ] ]" :=
+  (□ ∀ Φ, P -∗ (Q -∗ Φ pat%V) -∗ WP[W] e [{ Φ }])%I
+  (at level 20,
+   format "'[hv' [[{  '[' P  ']' } ] ] [ W ]  '/  ' e  '/' [[{  '[hv' RET  pat ;  '/' Q  ']' } ] ] ']'")
+  : bi_scope.
+Notation "[[{ P } ] ] [ W ] e ? [[{ 'RET' pat ; Q } ] ]" :=
+  (□ ∀ Φ, P -∗ (Q -∗ Φ pat%V) -∗ WP[W] e ?[{ Φ }])%I
+  (at level 20,
+   format "'[hv' [[{  '[' P  ']' } ] ] [ W ]  '/  ' e  '/' ? [[{  '[hv' RET  pat ;  '/' Q  ']' } ] ] ']'")
+  : bi_scope.
+
+(** Aliases for stdpp scope -- they inherit the levels and format from above. *)
+Notation "[[{ P } ] ] [ W ] e @ s ; E [[{ x .. y , 'RET' pat ; Q } ] ]" :=
+  (∀ Φ, P -∗ (∀ x, .. (∀ y, Q -∗ Φ pat%V) .. ) -∗ WP[W] e @ s; E [{ Φ }])
+  : stdpp_scope.
+Notation "[[{ P } ] ] [ W ] e @ E [[{ x .. y , 'RET' pat ; Q } ] ]" :=
+  (∀ Φ, P -∗ (∀ x, .. (∀ y, Q -∗ Φ pat%V) .. ) -∗ WP[W] e @ E [{ Φ }])
+  : stdpp_scope.
+Notation "[[{ P } ] ] [ W ] e @ E ? [[{ x .. y , 'RET' pat ; Q } ] ]" :=
+  (∀ Φ, P -∗ (∀ x, .. (∀ y, Q -∗ Φ pat%V) .. ) -∗ WP[W] e @ E ?[{ Φ }])
+  : stdpp_scope.
+Notation "[[{ P } ] ] [ W ] e [[{ x .. y , 'RET' pat ; Q } ] ]" :=
+  (∀ Φ, P -∗ (∀ x, .. (∀ y, Q -∗ Φ pat%V) .. ) -∗ WP[W] e [{ Φ }])
+  : stdpp_scope.
+Notation "[[{ P } ] ] [ W ] e ? [[{ x .. y , 'RET' pat ; Q } ] ]" :=
+  (∀ Φ, P -∗ (∀ x, .. (∀ y, Q -∗ Φ pat%V) .. ) -∗ WP[W] e ?[{ Φ }])
+  : stdpp_scope.
+Notation "[[{ P } ] ] [ W ] e @ s ; E [[{ 'RET' pat ; Q } ] ]" :=
+  (∀ Φ, P -∗ (Q -∗ Φ pat%V) -∗ WP[W] e @ s; E [{ Φ }]) : stdpp_scope.
+Notation "[[{ P } ] ] [ W ] e @ E [[{ 'RET' pat ; Q } ] ]" :=
+  (∀ Φ, P -∗ (Q -∗ Φ pat%V) -∗ WP[W] e @ E [{ Φ }]) : stdpp_scope.
+Notation "[[{ P } ] ] [ W ] e @ E ? [[{ 'RET' pat ; Q } ] ]" :=
+  (∀ Φ, P -∗ (Q -∗ Φ pat%V) -∗ WP[W] e @ E ?[{ Φ }]) : stdpp_scope.
+Notation "[[{ P } ] ] [ W ] e [[{ 'RET' pat ; Q } ] ]" :=
+  (∀ Φ, P -∗ (Q -∗ Φ pat%V) -∗ WP[W] e [{ Φ }]) : stdpp_scope.
+Notation "[[{ P } ] ] [ W ] e ? [[{ 'RET' pat ; Q } ] ]" :=
+  (∀ Φ, P -∗ (Q -∗ Φ pat%V) -∗ WP[W] e ?[{ Φ }]) : stdpp_scope.
