nola/examples/heap_lang/total_adequacy.v
@@ -6,8 +6,8 @@ From nola.examples.heap_lang Require Import proofmode notation.
 From iris.prelude Require Import options.
 
 Definition heap_total Σ `{!heapGpreS Σ} s e σ φ :
-  (∀ `{!heapGS_gen HasNoLc Σ}, ⊢ |==> ∃ W, let _ := HeapWGS _ W in
-    W ∗ (inv_heap_inv -∗ WP e @ s; ⊤ [{ v, ⌜φ v⌝ }])) →
+  (∀ `{!heapGS_gen HasNoLc Σ}, ⊢ |==> ∃ W,
+    W ∗ (inv_heap_inv -∗ WP[W] e @ s; ⊤ [{ v, ⌜φ v⌝ }])) →
   sn erased_step ([e], σ).
 Proof.
   intros Hwp; eapply (twp_total _ _); iIntros (?) "".
